Code/Syntax/Signature.v
@@ -1,3 +1,4 @@
+Require Import Prelude.Basics.
 Require Export Syntax.Signature.Types.
 Require Export Syntax.Signature.Contexts.
 Require Export Syntax.Signature.Terms.
@@ -6,28 +7,72 @@ Require Export Syntax.Signature.TermSubstitutions.
 Require Export Syntax.Signature.RewritingSystem.
 
 (** * The notion of Algebraic Functional System *)
-Record afs (B : Type) (F : Type) (R : Type) :=
-  {
-    Arity : F -> ty B ;
-    Vars : R -> con B ;
-    Tars : R -> B ;
-    Lhs : forall (r : R), tm Arity (Vars r) (Base (Tars r)) ;
-    Rhs : forall (r : R), tm Arity (Vars r) (Base (Tars r))
-  }.
+Record rewriteRule {B : Type} {F : Type} (ar : F -> ty B) :=
+  make_rewrite
+    {
+      Vars : con B ;
+      Tar : ty B ;
+      Lhs : tm ar Vars Tar ;
+      Rhs : tm ar Vars Tar
+    }.
 
-Arguments Arity {_ _ _}.
-Arguments Vars {_ _ _}.
-Arguments Tars {_ _ _}.
-Arguments Lhs {_ _ _}.
-Arguments Rhs {_ _ _}.
+Arguments make_rewrite {_ _ _} _ _ _ _.
+Arguments Vars {_ _ _} _.
+Arguments Tar {_ _ _} _.
+Arguments Lhs {_ _ _} _.
+Arguments Rhs {_ _ _} _.
+
+Record afs (B : Type) (F : Type) :=
+  make_afs
+    {
+      Arity : F -> ty B ;
+      RewriteRules : list (rewriteRule Arity)
+    }.
+
+Arguments make_afs {_ _} _ _.
+Arguments Arity {_ _} _ _.
+Arguments RewriteRules {_ _} _.
+
+Definition rewriteRules
+           {B F : Type}
+           (X : afs B F)
+  : Type
+  := members (RewriteRules X).
+
+Definition vars
+           {B F : Type}
+           {X : afs B F}
+           (r : rewriteRules X)
+  : con B
+  := Vars (member_el r).
+
+Definition tars
+           {B F : Type}
+           {X : afs B F}
+           (r : rewriteRules X)
+  : ty B
+  := Tar (member_el r).
+
+Definition lhs
+           {B F : Type}
+           {X : afs B F}
+           (r : rewriteRules X)
+  : tm (Arity X) (vars r) (tars r)
+  := Lhs (member_el r).
+
+Definition rhs
+           {B F : Type}
+           {X : afs B F}
+           (r : rewriteRules X)
+  : tm (Arity X) (vars r) (tars r)
+  := Rhs (member_el r).
 
 (** Accessor functions for AFSs *)
 Module AFSNotation.
   Definition tm
              {B : Type}
              {F : Type}
-             {R : Type}
-             (X : afs B F R)
+             (X : afs B F)
              (C : con B)
              (A : ty B)
   : Type
@@ -36,8 +81,7 @@ Module AFSNotation.
   Definition betaRed
              {B : Type}
              {F : Type}
-             {R : Type}
-             (X : afs B F R)
+             (X : afs B F)
              {C : con B}
              {A : ty B}
              (t1 t2 : tm X C A)
@@ -47,11 +91,9 @@ Module AFSNotation.
   Definition rew
              {B : Type}
              {F : Type}
-             {R : Type}
-             (X : afs B F R)
+             (X : afs B F)
              {C : con B}
              {A : ty B}
              (t1 t2 : tm X C A)
-    : Type
-    := RewritingSystem.rew (Lhs X) (Rhs X) t1 t2.
+    := RewritingSystem.rew lhs rhs t1 t2.
 End AFSNotation.
