Code/Preprocessing/PreprocessTerm.v
@@ -1,0 +1,129 @@
+Require Import Prelude.Basics.
+Require Import Preprocessing.TypeChecker.
+Require Import List.
+
+(** * Named terms *)
+
+(**
+The parser takes terms with named variables as input.
+Here we define such terms and we show how to map these to terms with De Bruijn indices.
+ *)
+Inductive rawNf (V F : Type) : Type :=
+| RawNeToNf : rawNe V F -> rawNf V F
+| RawNfLam : V -> rawNf V F -> rawNf V F
+with rawNe (V F : Type) : Type :=
+| RawNeVar : V -> rawNe V F
+| RawNeBase : F -> rawNe V F
+| RawNeApp : rawNe V F -> rawNf V F -> rawNe V F.
+
+Arguments RawNeToNf {_ _} _.
+Arguments RawNfLam {_ _} _ _.
+Arguments RawNeVar {_ _} _.
+Arguments RawNeBase {_ _} _.
+Arguments RawNeApp {_ _} _ _.
+
+(** Removing an element from the list *)
+Fixpoint remove
+         {A : Type}
+         `{decEq A}
+         (l : list A)
+         (a : A)
+  : list A
+  := match l with
+     | nil => nil
+     | x :: xs =>
+       match dec_eq x a with
+       | Yes _ => remove xs a
+       | No _ => x :: remove xs a
+       end
+     end.
+
+(** The free variables *)
+Fixpoint freeVarsNf
+         {V F : Type}
+         `{decEq V}
+         (t : rawNf V F)
+  : list V
+  := match t with
+     | RawNeToNf t => freeVarsNe t
+     | RawNfLam a t => remove (freeVarsNf t) a
+     end
+with freeVarsNe
+     {V F : Type}
+     `{decEq V}
+     (t : rawNe V F)
+  : list V
+  := match t with
+     | RawNeVar a => a :: nil
+     | RawNeBase b => nil
+     | RawNeApp t1 t2 => freeVarsNe t1 ++ freeVarsNf t2
+     end.
+
+(** Take the index of a variable *)
+Fixpoint rawVarToUtVar
+         {V : Type}
+         `{decEq V}
+         (vs : list V)
+         (x : V)
+  : option utVar
+  := match vs with
+     | nil => None
+     | v :: vs =>
+       match dec_eq x v with
+       | Yes _ => Some VzUt
+       | No _ =>
+         match rawVarToUtVar vs x with
+         | Some v' => Some (VsUt v')
+         | None => None
+         end
+       end
+     end.
+
+(** Go from terms with named variables to terms with De Bruijn indices *)
+Fixpoint rawNfToUtNf_vars
+         {V F : Type}
+         `{decEq V}
+         (vs : list V)
+         (t : rawNf V F)
+  : option (utNf F)
+  := match t with
+     | RawNeToNf t =>
+       match rawNeToUtNe_vars vs t with
+       | Some t' => Some (UtNeToNf t')
+       | None => None
+       end
+     | RawNfLam a t => rawNfToUtNf_vars (a :: vs) t
+     end
+with rawNeToUtNe_vars
+     {V F : Type}
+     `{decEq V}
+     (vs : list V)
+     (t : rawNe V F)
+  : option (utNe F)
+  := match t with
+     | RawNeVar v =>
+       match rawVarToUtVar vs v with
+       | Some t => Some (UtNeVar t)
+       | None => None
+       end
+     | RawNeBase f => Some (UtNeBase f)
+     | RawNeApp t1 t2 =>
+       match rawNeToUtNe_vars vs t1 , rawNfToUtNf_vars vs t2 with
+       | Some t1 , Some t2 => Some (UtNeApp t1 t2)
+       | _ , _ => None
+       end
+     end.
+
+Definition rawNfToUtNf
+           {V F : Type}
+           `{decEq V}
+           (t : rawNf V F)
+  : option (utNf F)
+  := rawNfToUtNf_vars (freeVarsNf t) t.
+
+Definition rawNfToUtNe
+           {V F : Type}
+           `{decEq V}
+           (t : rawNe V F)
+  : option (utNe F)
+  := rawNeToUtNe_vars (freeVarsNe t) t.
