Code/Preprocessing/Preprocessor.v
@@ -1,0 +1,435 @@
+Require Import Prelude.Funext.
+Require Import Prelude.Basics.
+Require Import Preprocessing.TypeChecker.
+Require Import Preprocessing.PreprocessTerm.
+Require Import Signature.
+Require Import List.
+Require Import Coq.Program.Equality.
+Require Import Prelude.Funext.
+
+(* For rewriting rules, use *)
+
+(** Help functions *)
+Definition dec_eq_members
+           {A : Type}
+           (l : list A)
+           `{decEq A}
+           (a1 a2 : members l)
+  : dec (a1 = a2).
+Proof.
+  destruct a1 as [a1 p1], a2 as [a2 p2].
+  destruct (dec_eq a1 a2) as [p | p].
+  - refine (Yes _).
+    abstract
+      (subst ;
+       f_equal ;
+       apply proof_irrelevance).
+  - refine (No _).
+    abstract
+      (intro q ;
+       inversion q ;
+       contradiction).
+Defined.
+
+Global Instance decEq_members
+       {A : Type}
+       (l : list A)
+       `{decEq A}
+  : decEq (members l)
+  := {| dec_eq := dec_eq_members l |}.
+
+Fixpoint list_option
+         {A : Type}
+         (l : list (option A))
+  : option (list A)
+  := match l with
+     | nil => Some nil
+     | x :: xs =>
+       match list_option xs with
+       | Some ys =>
+         match x with
+         | Some y => Some (y :: ys)
+         | None => None
+         end
+       | None => None
+       end
+     end.
+
+Definition decideIn
+           {A : Type}
+           `{decEq A}
+           (a : A)
+           (xs : list A)
+  : dec (In a xs).
+Proof.
+  induction xs as [ | x xs IHxs ].
+  - refine (No (fun q => _)).
+    abstract
+      (simpl in * ;
+       contradiction).
+  - destruct (dec_eq x a) as [ p | p ].
+    + refine (Yes _).
+      abstract
+        (left ;
+         exact p).
+    + destruct IHxs as [ q | q ].
+      * refine (Yes _).
+        abstract
+          (right ;
+           exact q).
+      * refine (No _).
+        abstract
+          (intro r ;
+           induction r ;
+           contradiction).
+Defined.
+
+Definition assocList
+           (A B : Type)
+  : Type
+  := list (A * B).
+
+Program Fixpoint getKey
+        {A B : Type}
+        `{decEq A}
+        (a : A)
+        (xs : assocList A B)
+  : option { b : B | In (pair a b) xs }
+  := match xs with
+     | nil => None
+     | (pair x b) :: xs =>
+       match dec_eq x a with
+       | Yes p => Some (exist _ b _)
+       | No p =>
+         match getKey a xs with
+         | Some (exist _ b' p) => Some (exist _ b' _)
+         | None => None
+         end
+       end
+     end.
+
+Definition not_hd_cons
+           {A : Type}
+           {a x : A}
+           {xs : list A}
+           (p : x <> a)
+           (q : In a (x :: xs))
+  : In a xs.
+Proof.
+  simpl in q.
+  destruct q ; try contradiction.
+  assumption.
+Qed.
+
+Definition fst_list
+           {A : Type}
+           {B : A -> Type}
+           (l : list { a : A & B a})
+  : list A
+  := map (@projT1 A B) l.
+
+Fixpoint dmap
+         {A : Type}
+         {B : A -> Type}
+         (f : forall (a : A), B a)
+         (l : list A)
+  : list { a : A & B a }
+  := match l with
+     | nil => nil
+     | x :: xs => (x , f x) :: dmap f xs
+     end.
+
+Fixpoint list_option_pair
+         {A : Type}
+         {B : A -> Type}
+         (l : list { a : A & option (B a) })
+  : option (list { a : A & B a })
+  := match l with
+     | nil => Some nil
+     | (x , Some p) :: xs =>
+       match list_option_pair xs with
+       | Some xs => Some ((x , p) :: xs)
+       | None => None
+       end
+     | (x , None) :: xs => None
+     end.
+
+Fixpoint list_to_map_el
+         {A : Type}
+         {B : A -> Type}
+         `{decEq A}
+         `{isFinite A}
+         (l : list { a : A & B a })
+  : forall (a : A), In a (fst_list l) -> B a
+  := match l with
+     | nil => fun a p => False_rect _ p
+     | (x , z) :: xs =>
+       fun a p =>
+         match dec_eq x a with
+         | Yes q => transport B q z
+         | No q => list_to_map_el xs a (not_hd_cons q p)
+         end
+     end.
+
+Definition list_to_map
+           {A : Type}
+           {B : A -> Type}
+           `{decEq A}
+           `{isFinite A}
+           (l : list { a : A & B a })
+           (p : forall (a : A), In a (fst_list l))
+  : forall (a : A), B a.
+Proof.
+  intro a.
+  specialize (p a).
+  exact (list_to_map_el _ _ p).
+Defined.
+
+Proposition in_dmap
+            {A : Type}
+            {B : A -> Type}
+            (f : forall (a : A), B a)
+            (xs : list A)
+            (a : A)
+            (p : In a xs)
+  : In a (fst_list (dmap f xs)).
+Proof.
+  induction xs as [ | x xs IHxs ] ; simpl in *.
+  - contradiction.
+  - destruct p as [ p | p ].
+    + left.
+      exact p.
+    + right.
+      apply IHxs.
+      exact p.
+Qed.
+
+Definition in_list_option_pair
+           {A : Type}
+           {B : A -> Type}
+           {l1 : list { a : A & option (B a) }}
+           {l2 : list { a : A & B a }}
+           (p : list_option_pair l1 = Some l2)
+           (a : A)
+           (q : In a (fst_list l1))
+  : In a (fst_list l2).
+Proof.
+  revert l2 p.
+  induction l1 as [ | x xs IHxs ] ; intros l2 p.
+  - simpl in *.
+    contradiction.
+  - simpl in *.
+    destruct x as [ x [ z | ]].
+    destruct (list_option_pair xs) as [ ys | ] ; simpl in *.
+    + inversion p.
+      subst ; simpl.
+      destruct q as [ q | q ].
+      * left.
+        exact q.
+      * right.
+        apply IHxs.
+        ** exact q.
+        ** reflexivity.
+    + discriminate.
+    + discriminate.
+Qed.
+
+Definition finite_option
+           {A : Type}
+           {B : A -> Type}
+           `{isFinite A}
+           `{decEq A}
+           (f : forall (a : A), option (B a))
+  : option (forall (a : A), B a).
+Proof.
+  pose (l := list_option_pair (dmap f els)).
+  assert (Hl : list_option_pair (dmap f els) = l) by reflexivity.
+  revert Hl.
+  destruct l as [ l | ] ; intros p.
+  - refine (Some _).
+    simple refine (list_to_map l _).
+    intro a.
+    apply (in_list_option_pair p).
+    apply in_dmap.
+    apply allIsMember.
+  - exact None.
+Defined.
+
+(** * The output of the parser *)
+Record parsedAFS (B V F : Type) : Type :=
+  {
+    TypeSymbols : list B ;
+    BaseTerms : assocList F (ty B) ;
+    FreeVars : assocList V (ty B) ;
+    Rewrites : list (rawNe V F * rawNf V F)
+  }.
+
+Arguments TypeSymbols {_ _ _} _.
+Arguments BaseTerms {_ _ _} _.
+Arguments FreeVars {_ _ _} _.
+Arguments Rewrites {_ _ _} _.
+
+(** Accessors for AFS *)
+Definition baseTypes
+           {B V F : Type}
+           (X : parsedAFS B V F)
+  : Type
+  := members (TypeSymbols X).
+
+Fixpoint to_baseType
+         {B V F : Type}
+         `{decEq B}
+         (X : parsedAFS B V F)
+         (A : ty B)
+  : option (ty (baseTypes X))
+  := match A with
+     | Base b =>
+       match decideIn b (TypeSymbols X) with
+       | Yes p => Some (Base (MakeMem b p))
+       | No p => None
+       end
+     | A1 ⟶ A2 =>
+       match to_baseType X A1 , to_baseType X A2 with
+       | Some A1 , Some A2 => Some (A1 ⟶ A2)
+       | _ , _ => None
+       end
+     end.
+
+(** * Processing to an AFS *)
+Definition afs_arity
+           {B V F : Type}
+           `{decEq B}
+           `{decEq F}
+           (X : parsedAFS B V F)
+  : option (members (BaseTerms X) -> ty (baseTypes X))
+  := finite_option (fun p => to_baseType X (snd (member_el p))).
+
+Fixpoint list_to_con
+         {B : Type}
+         (l : list (ty B))
+  : con B
+  := match l with
+     | nil => ∙
+     | x :: xs => x ,, list_to_con xs
+     end.
+
+Definition freeVars_to_con
+           {B V F : Type}
+           `{decEq B}
+           (X : parsedAFS B V F)
+  : option (con (baseTypes X))
+  := let l := map (fun z => to_baseType X (snd z)) (FreeVars X) in
+     match list_option l with
+     | Some tys => Some (list_to_con tys)
+     | None => None
+     end.
+
+Fixpoint check_functions_Nf
+         {B V F : Type}
+         `{decEq B}
+         `{decEq F}
+         `{decEq V}
+         (X : parsedAFS B V F)
+         (C : con (baseTypes X))
+         (ar : members (BaseTerms X) -> ty (baseTypes X))
+         (t : rawNf V F)
+  : option (rawNf V (members (BaseTerms X)))
+  := match t with
+     | RawNeToNf t =>
+       match check_functions_Ne X C ar t with
+       | Some t => Some (RawNeToNf t)
+       | None => None
+       end
+     | RawNfLam x t =>
+       match check_functions_Nf X C ar t with
+       | Some t => Some (RawNfLam x t)
+       | None => None
+       end
+     end
+with check_functions_Ne
+     {B V F : Type}
+     `{decEq B}
+     `{decEq F}
+     `{decEq V}
+     (X : parsedAFS B V F)
+     (C : con (baseTypes X))
+     (ar : members (BaseTerms X) -> ty (baseTypes X))
+     (t : rawNe V F)
+  : option (rawNe V (members (BaseTerms X)))
+  := match t with
+     | RawNeVar v => Some (RawNeVar v)
+     | RawNeBase f =>
+       match getKey f (BaseTerms X) with
+       | Some p => Some (RawNeBase (MakeMem (pair f (proj1_sig p)) (proj2_sig p)))
+       | None => None
+       end
+     | RawNeApp f t =>
+       match check_functions_Ne X C ar f , check_functions_Nf X C ar t with
+       | Some f , Some t => Some (RawNeApp f t)
+       | _ , _ => None
+       end
+     end.
+
+Definition to_rewriteRule
+           {B V F : Type}
+           `{decEq F}
+           `{decEq B}
+           `{decEq V}
+           {X : parsedAFS B V F}
+           (ar : members (BaseTerms X) -> ty (baseTypes X))
+           (t : rawNe V F * rawNf V F)
+  : option (rewriteRule ar)
+  := match t with
+     | pair t1 t2 =>
+       match freeVars_to_con X with
+       | Some C =>
+         match check_functions_Ne X C ar t1 with
+         | Some t1 =>
+           match rawNfToUtNe t1 with
+           | Some t1 =>
+             match infer_to_tm C ar t1 with
+             | Some (A , t1) =>
+               match check_functions_Nf X C ar t2 with
+               | Some t2 =>
+                 match rawNfToUtNf t2 with
+                 | Some t2 =>
+                   match check_to_tm C ar t2 A with
+                   | Some t2 => Some (make_rewrite C _ t1 t2)
+                   | None => None
+                   end
+                 | None => None
+                 end
+               | None => None
+               end
+             | None => None
+             end
+           | None => None
+           end
+         | None => None
+         end
+       | None => None
+       end
+     end.
+
+Definition parsedAFS_to_afs
+           {B V F : Type}
+           `{decEq B}
+           `{decEq F}
+           `{decEq V}
+           (X : parsedAFS B V F)
+  : option (afs (baseTypes X) (members (BaseTerms X)))
+  := match afs_arity X with
+     | Some ar =>
+       match freeVars_to_con X with
+       | Some C =>
+         match list_option (map (to_rewriteRule ar) (Rewrites X)) with
+         | Some rs => Some (make_afs ar rs)
+         | None => None
+         end
+       | None => None
+       end
+     | None => None
+     end.
+
+Require Import Extraction.
+Recursive Extraction parsedAFS_to_afs.
